theories/Math/OrderTheory.v
@@ -1,5 +1,9 @@
 Require Import PnV.Prelude.Prelude.
 
+#[local] Infix "\in" := E.In.
+#[local] Infix "\subseteq" := E.subset.
+#[local] Obligation Tactic := i.
+
 Lemma well_founded_implies_Irreflexive {A : Type} (R : A -> A -> Prop)
   (WF : well_founded R)
   : Irreflexive R.
@@ -7,28 +11,12 @@ Proof.
   intros x H_R. induction (WF x) as [x _ IH]. eapply IH with (y := x); exact H_R.
 Qed.
 
-Class has_ltProp (A : Type) : Type :=
-  { ltProp (lhs : A) (rhs : A) : Prop
-  ; ltProp_StrictOrder :: StrictOrder ltProp
-  }.
-
 #[program]
-Definition mkPosetFrom_ltProp {A : Type} (LTPROP : has_ltProp A) : isPoset A :=
+Definition mkPosetFrom_ltProp {A : Type} (ltProp : A -> A -> Prop) (ltProp_StrictOrder : StrictOrder ltProp) : isPoset A :=
   {| leProp x y := ltProp x y \/ x = y; Poset_isSetoid := mkSetoid_from_eq; |}.
 Next Obligation.
-  split; ii; firstorder try congruence. left. etransitivity; eauto.
+  split; ii; firstorder try congruence.
 Qed.
 Next Obligation.
-  destruct LTPROP as [lt [? ?]]. intros x y. cbn. unfold flip. cbv in StrictOrder_Irreflexive, StrictOrder_Transitive.
-  split; firstorder try congruence. contradiction (StrictOrder_Irreflexive x). firstorder.
+  intros x y. cbn. unfold flip. split; firstorder try congruence. contradiction (StrictOrder_Irreflexive x). firstorder.
 Qed.
-
-Class hasSimulation (Src : Type) (Tgt : Type) {Src_isPoset : isPoset Src} {Tgt_isPoset : isPoset Tgt} : Type :=
-  { simulation : Src -> Tgt
-  ; simulation_compatWith_eqProp :: eqPropCompatible1 simulation
-  ; simulation_spec s t'
-    : (exists t, simulation s =< t /\ t == t') <-> (exists s', s =< s' /\ simulation s' == t')
-  }.
-
-Class isWellPreOrderedSet (A : Type) (leProp : A -> A -> Prop) {PREORDER : PreOrder leProp} : Type :=
-  wellorder (x : nat -> A) : { '(i, j) : nat * nat | i < j /\ leProp (x i) (x j) }.
